More debugging

rupicola/io/RunningExample.fst
@@ -35,14 +35,23 @@ let good_agent fn task =
 let test () =
   wrapper "bla" "st" good_agent
 
-[@expect_failure]
-%splice_t[tgt_test] (meta_translation "tgt_test" [`test])
-
-[@expect_failure]
-%splice_t[tgt_wrapper] (meta_translation "tgt_wrapper" [`wrapper])
-
 let simpler_test () =
   let!@! contents = read_file "todo" in
   io_return (Inl ())
 
-%splice_t[tgt_test] (meta_translation "tgt_test" [`simpler_test])
+val ignore_io : io 'a -> unit
+let ignore_io m = ()
+
+let ignored_test () =
+  ignore_io (simpler_test ())
+
+[@expect_failure]
+%splice_t[tgt_test] (meta_translation "tgt_test" [`ignored_test])
+
+// %splice_t[tgt_test] (meta_translation "tgt_test" [`simpler_test])
+
+// [@expect_failure]
+// %splice_t[tgt_wrapper] (meta_translation "tgt_wrapper" [`wrapper])
+
+// [@expect_failure]
+// %splice_t[tgt_test] (meta_translation "tgt_test" [`test])
